# 14.3 Partial Derivatives
2023-04-15 | 00:45
{Subject}:[[MTHS 211]]
{Section}:[[14.0 Partial Derivatives]]
{Tags}: #Mathematics #Calculus 
{Related}:

--- 
### Definition
If $f$ is a function of two variables, its partial derivatives are the functions $f_x$ and $f_y$ defined by
$$
\begin{aligned}
f_x(x, y) & =\lim _{h \rightarrow 0} \frac{f(x+h, y)-f(x, y)}{h} \\
f_y(x, y) & =\lim _{h \rightarrow 0} \frac{f(x, y+h)-f(x, y)}{h}
\end{aligned}
$$

---
Notations for Partial Derivatives If $z=f(x, y)$, we write
$$
\begin{aligned}
& f_x(x, y)=f_x=\frac{\partial f}{\partial x}=\frac{\partial}{\partial x} f(x, y)=\frac{\partial z}{\partial x}=f_1=D_1 f=D_x f \\
& f_y(x, y)=f_y=\frac{\partial f}{\partial y}=\frac{\partial}{\partial y} f(x, y)=\frac{\partial z}{\partial y}=f_2=D_2 f=D_y f
\end{aligned}
$$
Rule for Finding Partial Derivatives of $z=f(x, y)$
1. To find $f_x$, regard $y$ as a constant and differentiate $f(x, y)$ with respect to $x$.
2. To find $f_y$, regard $x$ as a constant and differentiate $f(x, y)$ with respect to $y$.

---
### Clairaut's Theorem

Suppose $f$ is defined on a disk $D$ that contains the point $(a, b)$. If the functions $f_{x y}$ and $f_{y x}$ are both continuous on $D$, then $f_{x y}(a, b)=f_{y x}(a, b)$.

---
Proof. For small values of $h, h \neq 0$, consider the difference
$$
\Delta(h)=[f(a+h, b+h)-f(a+h, b)]-[f(a, b+h)-f(a, b)]
$$
If we let $g(x)=f(x, b+h)-f(x, b)$, then
$$
\Delta(h)=g(a+h)-g(a)
$$
Note that if $g(c)=f(c, b+h)-f(c, b)$ then $g^{\prime}(c)=f_x(c, b+h)-f_x(c, b)$. By the Mean Value Theorem, there is a nuber $c \in(a, a+h)$ such that
$$
\Delta(h)=g(a+h)-g(a)=g^{\prime}(c) h=h\left[f_x(c, b+h)-f_x(c, b)\right]
$$
Again using the Mean Value Theorem, this time to the function $f_x$, we can find a number $d \in(b, b+h)$ such that
$$
f_x(c, b+h)-f_x(c, b)=f_{x y}(c, d) h
$$
Combining the equations we get
$$
\Delta(h)=h^2 f_{x y}(c, d)
$$
If $h \rightarrow 0$, then $(c, d) \rightarrow(a, b)$. so the continuity of $f_{x y}$ at $(a, b)$ gives
$$
\lim _{h \rightarrow 0} \frac{\Delta(h)}{h^2}=\lim _{(c, d) \rightarrow(a, b)} f_{x y}(c, d)=f_{x y}(a, b) .
$$
Similarly, we can write $\Delta(h)$ as
$$
\Delta(h)=[f(a+h, b+h)-f(a, b+h)]-[f(a+h, b)-f(a, b)]
$$
and using the Mean Value Theorem twice and the continuity of $f_{y x}$ at $(a, b)$, we obtain
$$
\lim _{h \rightarrow 0} \frac{\Delta(h)}{h^2}=f_{y x}(a, b) .
$$
It follows that $f_{x y}(a, b)=f_{y x}(a, b)$.
--- 
{Efundi Lecture Notes}:https://efundi.nwu.ac.za/access/content/group/4c4529f0-7790-4dc7-9390-8f7cd29c9a77/2021/English/Lecture%20Notes/MTHS211%20-%20Lecture%206%20-%20Partial%20Derivatives.pdf