17:41# 3.7 Ordered Statistics
2023-04-25 | 21:13
{Subject}:[[STTN 215]]
{Section}:[[03 Joint Distributions]]
{Tags}: #Probability 
{Related}:

--- 
 Suppose

### Definition

The random variables $X_1,\dots,X_n$ are `Identically distributed` if they all share the same density function (or mass function):

$$
\large
\therefore f_{X_i}(t)=f(t) \hspace{1 cm} \forall \hspace{1 cm} i=1,\dots,n 
$$
$$\large
p_{X_i}(k)=p(k) \hspace{1 cm} \forall \hspace{1 cm} i=1,\dots,n $$

### Definition

Suppose $X_1,\dots,X_n$ are $n$ random variables and they are sorted from smallest to biggest. This ordering will be denoted by: $X_{(1)}\le X_{(2)}\le \dots \le X_{(n)}$. In other words $X_{(1)} = min(X_1,\dots,X_n)$ and $X_{(n)} = max(X_1,\dots,X_n)$.
We say that $X_{(1)}\le X_{(2)}\le \dots \le X_{(n)}$ are the ordered statistics of $X_1,\dots,X_n$.

### Theorem 3.3

Let $f_{X_{(n)}}(x)$ be the density function of $X_{(n)}$. Then:

$$\large f_{X_{(n)}}(x)=n\{F(x)\}^{n-1}f(x) $$

---
Proof:

$$
\large
\begin{align}
F_{X_{(n)}}(x) &=P(X_{(n)}\le x) \\
&=P(max(X_1,\dots,X_n)\le x) \\
&=P(X_1\le x,X_2\le x,\dots,X_n\le x) \\
&=P(X_1\le x)P(X_2\le x)\dots P(X_n\le x) \\
&=F(X).F(X)\dots F(X) \\
&=(F(X))^n \\
&\text{Differentiate on both sides to x:} \\
&\therefore f_{X_{(n)}}(x)=n\{F(x)\}^{n-1}f(x)
\end{align}
$$

---
### Theorem 3.4

Let $f_{X_{(1)}}(x)$ be the density function of $X_{(1)}$. Then

$$ f_{X_{(1)}}(x)=n\{1-F(x)\}^{n-1}f(x) $$

---

Proof:

$$
\large
\begin{align}
F_{X_{(1)}}(x)&=P(X_{(1)}\le x) \\
&=1-P(X_{(1)}> x) \\
&=1-P(X_{1}> x,X_{2}> x,\dots,X_{n}> x) \\
&=1-P(X_{1}> x).P(X_{2}> x)\dots P(X_{n}> x)\\
&=1-(1-P(X_{1}\le x))(1-P(X_{2}\le x))\dots(1-P(X_{n}\le x))\\
&=1-(1-F(x))(1-F(x))\dots(1-F(x))\\
&=1-(1-F(x))^n\\
&\text{Differentiate on both sides to x:}\\
&f_{X_{(1)}}(x)=-n(1-F(x))^{n-1}(-f(x))\\
&=n(1-F(x))^{n-1}f(x)
\end{align}
$$

---
**Theorem 3.5**
Let $f_{X_{(k)}}(x)$ be the density function of $X_{(k)}$, for $k=1,2,\dots,n$. Then we have:
$$
\large
f_{X_{(k)}}(x)=\frac{n!}{(k-1)!(n-k)!}\{F(x)\}^{k-1}\{1-F(x)\}^{n-k}f(x)
$$

---
**Remark 2**
Hence we obtain an easy method to determine integrals of the form $\int^1_0x^{\alpha-1}(1-x)^{\beta-1}dx$
$$
\int^1_0x^{\alpha-1}(1-x)^{\beta-1}dx = \frac{\Gamma(\alpha)\Gamma(\beta)}{\Gamma(\alpha+\beta)}
$$



--- 
{Efundi Lecture Notes}: [Ordered Statistics](https://efundi.nwu.ac.za/access/content/group/60117479-9808-427c-89ba-453cd261722f/SLIDES/STTN215_Chapter3_Joint_Distributions_2021.pdf)